fix sorts

src/Theories/Sorts.v
@@ -34,13 +34,34 @@ Section sorts.
     @patt_sym sig (inj s).
   
   Example test_pattern_1 := patt_equal (sym inhabitant) (sym inhabitant).
-  Definition inhabitant_set(phi : Pattern) : Pattern := sym inhabitant $ phi.
+  Definition patt_inhabitant_set(phi : Pattern) : Pattern := sym inhabitant $ phi.
+
+
+  Lemma evar_open_inhabitant_set db x ϕ :
+    evar_open db x (patt_inhabitant_set ϕ) = patt_inhabitant_set (evar_open db x ϕ).
+  Proof. unfold patt_inhabitant_set. rewrite !simpl_evar_open. reflexivity. Qed.
+  
+  Lemma svar_open_inhabitant_set db x ϕ :
+    svar_open db x (patt_inhabitant_set ϕ) = patt_inhabitant_set (svar_open db x ϕ).
+  Proof. unfold patt_inhabitant_set. rewrite !simpl_svar_open. reflexivity. Qed.
+  
+  #[global]
+   Instance Unary_inhabitant_set : Unary patt_inhabitant_set :=
+    {| unary_evar_open := evar_open_inhabitant_set ;
+       unary_svar_open := svar_open_inhabitant_set ;
+    |}.
+
+  Class PSort (patt_sort : Pattern) :=
+    { (*patt_sort : Pattern ;*)
+      psort_closed : free_evars patt_sort = ∅ ;
+      psort_wfc : well_formed_closed patt_sort ;
+    }.
 
   Definition patt_forall_of_sort (sort phi : Pattern) : Pattern :=
-    patt_forall ((patt_in (patt_bound_evar 0) (inhabitant_set sort)) ---> phi).
+    patt_forall ((patt_in (patt_bound_evar 0) (patt_inhabitant_set sort)) ---> phi).
 
   Definition patt_exists_of_sort (sort phi : Pattern) : Pattern :=
-    patt_exists ((patt_in (patt_bound_evar 0) (inhabitant_set sort)) and phi).
+    patt_exists ((patt_in (patt_bound_evar 0) (patt_inhabitant_set sort)) and phi).
 
   (* TODO patt_forall_of_sort and patt_exists_of_sorts are duals - a lemma *)
 
@@ -56,36 +77,29 @@ Section sorts.
     Context {M : Model}.
     Hypothesis M_satisfies_theory : M ⊨ᵀ Definedness.theory.
 
-    Definition Minhabitant_set m := app_ext (sym_interp (inj inhabitant)) (Ensembles.Singleton (Domain M) m).
+    Definition Mpatt_inhabitant_set m := app_ext (sym_interp (inj inhabitant)) (Ensembles.Singleton (Domain M) m).
 
     (* ϕ is expected to be a sort pattern *)
-    Definition Minterp_inhabitant ϕ ρₑ ρₛ := @pattern_interpretation sig M ρₑ ρₛ (patt_app (sym inhabitant) ϕ).
-
-
-    Class PSort :=
-      { patt_sort : Pattern ;
-        patt_sort_closed : free_evars patt_sort = ∅ ;
-        patt_sort_wfc : well_formed_closed patt_sort ;
-      }.
+    Definition Minterp_inhabitant ϕ ρₑ ρₛ := @pattern_interpretation sig M ρₑ ρₛ (patt_app (sym inhabitant) ϕ).    
     
-    
-    Lemma pattern_interpretation_forall_of_sort_predicate (s : PSort) ϕ ρₑ ρₛ:
+    Lemma pattern_interpretation_forall_of_sort_predicate s (Hpss : PSort s) ϕ ρₑ ρₛ:
       let x := fresh_evar ϕ in
       M_predicate M (evar_open 0 x ϕ) ->
-      pattern_interpretation ρₑ ρₛ (patt_forall_of_sort (@patt_sort s) ϕ) = Full
-      <-> (∀ m : Domain M, Minterp_inhabitant (@patt_sort s) ρₑ ρₛ m ->
+      pattern_interpretation ρₑ ρₛ (patt_forall_of_sort s ϕ) = Full
+      <-> (∀ m : Domain M, Minterp_inhabitant s ρₑ ρₛ m ->
                            pattern_interpretation (update_evar_val x m ρₑ) ρₛ (evar_open 0 x ϕ) = Full).
     Proof.
       intros x Hpred.
       unfold patt_forall_of_sort.
-      assert (Hfr: fresh_evar (patt_in b0 (inhabitant_set patt_sort) ---> ϕ) = fresh_evar ϕ).
+      assert (Hfr: fresh_evar (patt_in b0 (patt_inhabitant_set s) ---> ϕ) = fresh_evar ϕ).
       { unfold fresh_evar. apply f_equal. apply f_equal. simpl.
-        rewrite -> patt_sort_closed.
+        rewrite -> psort_closed.
         repeat rewrite -> sets.union_empty_l_L.
         auto.
       }
       rewrite pattern_interpretation_forall_predicate.
       2: {
+        (*rewrite !simpl_evar_open.*)
         autorewrite with ml_db.
         simpl.
         apply M_predicate_impl.
@@ -103,16 +117,16 @@ Section sorts.
         rewrite -> Hfr in H.
         eapply pattern_interpretation_impl_MP. apply H.
         unfold Minterp_inhabitant in H'.
-        pose proof (Hfeip := @free_evar_in_patt _ _ M M_satisfies_theory (fresh_evar ϕ) (patt_sym (inj inhabitant) $ evar_open 0 (fresh_evar ϕ) patt_sort) (update_evar_val (fresh_evar ϕ) m ρₑ) ρₛ).
+        pose proof (Hfeip := @free_evar_in_patt _ _ M M_satisfies_theory (fresh_evar ϕ) (patt_sym (inj inhabitant) $ evar_open 0 (fresh_evar ϕ) s) (update_evar_val (fresh_evar ϕ) m ρₑ) ρₛ).
         destruct Hfeip as [Hfeip1 _]. apply Hfeip1. clear Hfeip1.
         rewrite update_evar_val_same.
         clear H. unfold sym in H'.
         unfold Ensembles.In.
-        rewrite -> evar_open_wfc. 2: apply patt_sort_wfc.
+        rewrite -> evar_open_wfc. 2: apply psort_wfc.
         rewrite -> pattern_interpretation_free_evar_independent.
         3: { intros Contra. simpl in Contra.
              rewrite -> sets.union_empty_l_L in Contra.
-             rewrite -> patt_sort_closed in Contra.
+             rewrite -> psort_closed in Contra.
              apply base.not_elem_of_empty in Contra.
              apply Contra.
         }
@@ -120,12 +134,12 @@ Section sorts.
              constructor.
              constructor.
              apply wfc_wfc_ind.
-             apply patt_sort_wfc.
+             apply psort_wfc.
         }
         apply H'.
       - intros H m.
         autorewrite with ml_db. simpl.
-        pose proof (Hfeip := @free_evar_in_patt _ _ M M_satisfies_theory (fresh_evar ϕ) (patt_sym (inj inhabitant) $ evar_open 0 (fresh_evar ϕ) patt_sort) (update_evar_val (fresh_evar ϕ) m ρₑ) ρₛ).
+        pose proof (Hfeip := @free_evar_in_patt _ _ M M_satisfies_theory (fresh_evar ϕ) (patt_sym (inj inhabitant) $ evar_open 0 (fresh_evar ϕ) s) (update_evar_val (fresh_evar ϕ) m ρₑ) ρₛ).
         destruct Hfeip as [_ Hfeip2].
         apply pattern_interpretation_predicate_impl.
         apply T_predicate_in. apply M_satisfies_theory.
@@ -133,12 +147,12 @@ Section sorts.
         specialize (Hfeip2 H1). clear H1.
         apply H. unfold Minterp_inhabitant.
         unfold Ensembles.In in Hfeip2. unfold sym.
-        rewrite -> evar_open_wfc in Hfeip2. 2: apply patt_sort_wfc.
+        rewrite -> evar_open_wfc in Hfeip2. 2: apply psort_wfc.
         rewrite -> update_evar_val_same in Hfeip2.
         rewrite -> pattern_interpretation_free_evar_independent in Hfeip2.
         3: { intros Contra. simpl in Contra.
              rewrite -> sets.union_empty_l_L in Contra.
-             rewrite -> patt_sort_closed in Contra.
+             rewrite -> psort_closed in Contra.
              apply base.not_elem_of_empty in Contra.
              apply Contra.
         }
@@ -146,23 +160,23 @@ Section sorts.
              constructor.
              constructor.
              apply wfc_wfc_ind.
-             apply patt_sort_wfc.
+             apply psort_wfc.
         }
         apply Hfeip2.
     Qed.
 
-    Lemma pattern_interpretation_exists_of_sort_predicate (s : PSort) ϕ ρₑ ρₛ:
+    Lemma pattern_interpretation_exists_of_sort_predicate s (Hpss : PSort s) ϕ ρₑ ρₛ:
       let x := fresh_evar ϕ in
       M_predicate M (evar_open 0 x ϕ) ->
-      pattern_interpretation ρₑ ρₛ (patt_exists_of_sort patt_sort ϕ) = Full
-      <-> (∃ m : Domain M, Minterp_inhabitant patt_sort ρₑ ρₛ m /\
+      pattern_interpretation ρₑ ρₛ (patt_exists_of_sort s ϕ) = Full
+      <-> (∃ m : Domain M, Minterp_inhabitant s ρₑ ρₛ m /\
                            pattern_interpretation (update_evar_val x m ρₑ) ρₛ (evar_open 0 x ϕ) = Full).
     Proof.
       intros x Hpred.
       unfold patt_exists_of_sort.
-      assert (Hfr: fresh_evar (patt_in b0 (inhabitant_set patt_sort) and ϕ) = fresh_evar ϕ).
+      assert (Hfr: fresh_evar (patt_in b0 (patt_inhabitant_set s) and ϕ) = fresh_evar ϕ).
       { unfold fresh_evar. apply f_equal. apply f_equal. simpl.
-        rewrite -> patt_sort_closed.
+        rewrite -> psort_closed.
         repeat rewrite -> sets.union_empty_r_L.
         rewrite -> sets.union_empty_l_L.
         auto.
@@ -187,16 +201,16 @@ Section sorts.
         destruct H as [H1 H2].
         exists m. split. 2: apply H2. clear H2.
         unfold Minterp_inhabitant.
-        pose proof (Hfeip := @free_evar_in_patt _ _ M M_satisfies_theory (fresh_evar ϕ) (patt_sym (inj inhabitant) $ evar_open 0 (fresh_evar ϕ) patt_sort) (update_evar_val (fresh_evar ϕ) m ρₑ) ρₛ).
+        pose proof (Hfeip := @free_evar_in_patt _ _ M M_satisfies_theory (fresh_evar ϕ) (patt_sym (inj inhabitant) $ evar_open 0 (fresh_evar ϕ) s) (update_evar_val (fresh_evar ϕ) m ρₑ) ρₛ).
         destruct Hfeip as [_ Hfeip2]. apply Hfeip2 in H1. clear Hfeip2.
         rewrite update_evar_val_same in H1.
         unfold sym.
         unfold Ensembles.In in H1.
-        rewrite -> evar_open_wfc in H1. 2: apply patt_sort_wfc.
+        rewrite -> evar_open_wfc in H1. 2: apply psort_wfc.
         rewrite -> pattern_interpretation_free_evar_independent in H1.
         3: { intros Contra. simpl in Contra.
              rewrite -> sets.union_empty_l_L in Contra.
-             rewrite -> patt_sort_closed in Contra.
+             rewrite -> psort_closed in Contra.
              apply base.not_elem_of_empty in Contra.
              apply Contra.
         }
@@ -204,12 +218,12 @@ Section sorts.
              constructor.
              constructor.
              apply wfc_wfc_ind.
-             apply patt_sort_wfc.
+             apply psort_wfc.
         }
         apply H1.
       - intros [m [H1 H2]]. exists m.
         autorewrite with ml_db. simpl.
-        pose proof (Hfeip := @free_evar_in_patt _ _ M M_satisfies_theory (fresh_evar ϕ) (patt_sym (inj inhabitant) $ evar_open 0 (fresh_evar ϕ) patt_sort) (update_evar_val (fresh_evar ϕ) m ρₑ) ρₛ).
+        pose proof (Hfeip := @free_evar_in_patt _ _ M M_satisfies_theory (fresh_evar ϕ) (patt_sym (inj inhabitant) $ evar_open 0 (fresh_evar ϕ) s) (update_evar_val (fresh_evar ϕ) m ρₑ) ρₛ).
         destruct Hfeip as [Hfeip1 _].
         apply pattern_interpretation_and_full.
         rewrite -> Hfr.
@@ -218,11 +232,11 @@ Section sorts.
           unfold Ensembles.In.
           rewrite -> update_evar_val_same.
           unfold Minterp_inhabitant in H1. unfold sym in H1.
-          rewrite -> evar_open_wfc. 2: apply patt_sort_wfc.
+          rewrite -> evar_open_wfc. 2: apply psort_wfc.
           rewrite -> pattern_interpretation_free_evar_independent.
           3: { intros Contra. simpl in Contra.
                rewrite -> sets.union_empty_l_L in Contra.
-               rewrite -> patt_sort_closed in Contra.
+               rewrite -> psort_closed in Contra.
                apply base.not_elem_of_empty in Contra.
                apply Contra.
           }
@@ -230,16 +244,16 @@ Section sorts.
                constructor.
                constructor.
                apply wfc_wfc_ind.
-               apply patt_sort_wfc.
+               apply psort_wfc.
           }
           apply H1.
         + apply H2.
     Qed.
 
 
-    Lemma M_predicate_exists_of_sort (s : PSort) ϕ :
+    Lemma M_predicate_exists_of_sort s (Hpss : PSort s) ϕ :
       let x := fresh_evar ϕ in
-      M_predicate M (evar_open 0 x ϕ) -> M_predicate M (patt_exists_of_sort patt_sort ϕ).
+      M_predicate M (evar_open 0 x ϕ) -> M_predicate M (patt_exists_of_sort s ϕ).
     Proof.
       intros x Hpred.
       unfold patt_exists_of_sort.
@@ -249,7 +263,7 @@ Section sorts.
       - apply T_predicate_in.
         apply M_satisfies_theory.
       - simpl.
-        rewrite -> patt_sort_closed.
+        rewrite -> psort_closed.
         repeat rewrite sets.union_empty_r_L.
         repeat rewrite sets.union_empty_l_L.
         subst x.
@@ -257,9 +271,9 @@ Section sorts.
         apply Hpred.
     Qed.
 
-    Lemma M_predicate_forall_of_sort (s : PSort) ϕ :
+    Lemma M_predicate_forall_of_sort s (Hpss : PSort s) ϕ :
       let x := fresh_evar ϕ in
-      M_predicate M (evar_open 0 x ϕ) -> M_predicate M (patt_forall_of_sort patt_sort ϕ).
+      M_predicate M (evar_open 0 x ϕ) -> M_predicate M (patt_forall_of_sort s ϕ).
     Proof.
       intros x Hpred.
       unfold patt_forall_of_sort.
@@ -269,7 +283,7 @@ Section sorts.
       - apply T_predicate_in.
         apply M_satisfies_theory.
       - simpl.
-        rewrite -> patt_sort_closed.
+        rewrite -> psort_closed.
         rewrite !(@right_id _ (=) ∅ (∪) ).
         rewrite (@left_id _ (=) ∅).
         subst x.
@@ -278,12 +292,12 @@ Section sorts.
     Qed.
 
     
-    Lemma interp_total_function f (s₁ s₂ : PSort) ρₑ ρₛ :
-      @pattern_interpretation sig M ρₑ ρₛ (patt_total_function f (@patt_sort s₁) (@patt_sort s₂)) = Full ->
+    Lemma interp_total_function f s₁ s₂ (Hpss₁ : PSort s₁) (Hpss₂ : PSort s₂) ρₑ ρₛ :
+      @pattern_interpretation sig M ρₑ ρₛ (patt_total_function f s₁ s₂) = Full ->
       ∀ (m₁ : Domain M),
-        Minterp_inhabitant (@patt_sort s₁) ρₑ ρₛ m₁ ->                 
+        Minterp_inhabitant s₁ ρₑ ρₛ m₁ ->                 
         ∃ (m₂ : Domain M),
-          Minterp_inhabitant (@patt_sort s₂) ρₑ ρₛ m₂ ->
+          Minterp_inhabitant s₂ ρₑ ρₛ m₂ ->
           app_ext (@pattern_interpretation sig M ρₑ ρₛ f) (Ensembles.Singleton (Domain M) m₁)
           = Ensembles.Singleton (Domain M) m₂.
     Proof.
